"Proof of Fp2_correct automated"

src/Bedrock/Field/Synthesis/Examples/quadratic_extension_bls12.v
@@ -82,8 +82,6 @@ Require Import Crypto.Bedrock.Field.Synthesis.Examples.bls12prime.
 Local Open Scope Z_scope.
 
 (*Parameters to be changed: specify prime and import reification from cache.*)
-    Local Definition u := -0xd201000000010000.
-    Local Definition p_of_u u := (((u - 1)^2 * (u^4 - u^2 + 1)) / 3) + u.
     Local Notation m := bls12prime.m.
     Local Definition prefix := "bls12_"%string. (* placed before function names *)
 
@@ -95,10 +93,10 @@ Local Open Scope Z_scope.
     Change names to match reification cache.*)
     Lemma m_eq: bls12prime.m = m.
     Proof.
-        unfold m. unfold bls12prime.m. reflexivity.
+        unfold m. reflexivity.
     Qed.
 (*  We instantiate specs of all imported bedrock2 functions.
-    This needs to be done for typeclass inference to wrok properly.*)
+    This needs to be done for typeclass inference to work properly.*)
 
   Instance spec_of_reified_mul :
   spec_of (append prefix "mul") := spec_of_mul.
@@ -145,6 +143,8 @@ Local Definition valid_words w := valid (List.map Interface.word.unsigned w).
 Local Definition map_words := List.map Interface.word.unsigned.
 Local Notation r := (WordByWordMontgomery.r bw).
 Local Notation r' := (WordByWordMontgomery.r' m bw).
+Local Definition num_bytes := Eval compute in (Z.of_nat (((Z.to_nat bw * n) / 8)%nat)).
+
 
 Lemma bw_eq : WordByWordMontgomery.n m (@width (@semantics Defaults64.default_parameters)) = n.
 Proof.
@@ -204,9 +204,9 @@ Definition Fp2_mul_Gallina_spec in1 in2 out :=
     ("Fp2_mul", (
       [outr; outi; xr; xi; yr; yi], [],
       bedrock_func_body:(
-      stackalloc 48 as v0 {
-        stackalloc 48 as v1 {
-          stackalloc 48 as v2 {
+      stackalloc num_bytes as v0 {
+        stackalloc num_bytes as v1 {
+          stackalloc num_bytes as v2 {
             mul (v0, xr, yr);
             mul (v1, xi, yi);
             sub (outr, v0, v1);
@@ -220,7 +220,7 @@ Definition Fp2_mul_Gallina_spec in1 in2 out :=
       }
       )
     )).
-
+    
   Local Open Scope string_scope.
   Local Infix "*" := sep : sep_scope.
   Delimit Scope sep_scope with sep.
@@ -292,8 +292,6 @@ fun functions : list (string * (list string * list string * cmd)) =>
 Require Import Crypto.Bedrock.Field.Synthesis.Specialized.Tactics.
 Require Import bedrock2.string2ident.
 Require Import Crypto.Arithmetic.WordByWordMontgomery.
-
-
 Require Import bedrock2.Map.SeparationLogic.
 Require Import coqutil.Tactics.syntactic_unify.
 Require Import bedrock2.Lift1Prop.
@@ -351,61 +349,18 @@ Proof.
     - pose proof (WordByWordMontgomery.from_montgomerymod_correct bw n m r' m').
       apply (H0).
       all: (auto; simpl; try lia).
-        + unfold m. lia.
+        + unfold m. simpl. lia.
         + unfold m. cbv [WordByWordMontgomery.n]. simpl. lia.
-        + unfold m. lia.
+        + unfold m. simpl. lia.
     - destruct H0. rewrite Z.mod_small; try reflexivity. unfold eval. auto.
 Qed.
 
-Check Interface.map.split.
+(*In order to prove the correctness of Fp2_mul, some automation is in order
+  We start with a couple of technical lemmas.*)
 Notation msplit := Interface.map.split.
 
-Lemma split_split_split : forall (m m1 m2 x0 x1 : @Interface.map.rep (@word (@semantics Defaults64.default_parameters))
-Init.Byte.byte (@mem (@semantics Defaults64.default_parameters))), msplit m m1 m2 -> msplit m1 x0 x1
-  -> msplit m (Interface.map.putmany m2 x1) x0.
-Proof.
-  intros. split.
-    - pose proof Properties.map.putmany_assoc.
-      destruct H. destruct H0. rewrite H. rewrite H0. rewrite (Properties.map.putmany_comm x0 x1); auto.
-      rewrite (Properties.map.putmany_comm).
-
-      + rewrite Properties.map.putmany_assoc; auto.
-        * rewrite Properties.map.disjoint_comm. apply Properties.map.sub_domain_disjoint with (m1' := m1); auto.
-          rewrite H0. rewrite Properties.map.putmany_comm; auto.
-          apply Properties.map.sub_domain_putmany_r. apply Properties.map.sub_domain_refl.
-        * apply Properties.map.disjoint_comm. auto.
-        * rewrite Properties.map.disjoint_comm. apply Properties.map.sub_domain_disjoint with (m1' := m1); auto.
-          rewrite H0. apply Properties.map.sub_domain_putmany_r. apply Properties.map.sub_domain_refl.
-      + rewrite Properties.map.putmany_comm.
-        * rewrite <- H0; auto.
-        * rewrite Properties.map.disjoint_comm. auto.
-  - destruct H, H0. apply Properties.map.disjoint_putmany_l. split.
-    + rewrite Properties.map.disjoint_comm. apply Properties.map.sub_domain_disjoint with (m1' := m1); auto.
-      rewrite H0. apply Properties.map.sub_domain_putmany_r. apply Properties.map.sub_domain_refl.
-    + apply Properties.map.disjoint_comm; auto.
-Qed.
-
- Definition R_putmany (m1 m2 m : @Interface.map.rep (@word (@semantics Defaults64.default_parameters))
- Init.Byte.byte (@mem (@semantics Defaults64.default_parameters))) := m = Interface.map.putmany m1 m2.
-    
-Lemma alloc_seps (m m1 m2 : @Interface.map.rep (@word (@semantics Defaults64.default_parameters))
-Init.Byte.byte (@mem (@semantics Defaults64.default_parameters)))
- P : Interface.map.split m m1 m2 -> (exists R, (P * R)%sep m1) ->
-  exists (R' : Interface.map.rep -> Prop), (P * R')%sep m.
-Proof.
-  intros. destruct H0. destruct H0. destruct H0. destruct H0. destruct H1.
-   exists (R_putmany x1 m2). unfold sep. exists x0. exists (Interface.map.putmany x1 m2).
-    split.
-      - rewrite Properties.map.split_comm. rewrite Properties.map.putmany_comm.
-        + apply (split_split_split m m1 m2 x0 x1 H H0).
-        + destruct H. apply Properties.map.sub_domain_disjoint with (m1' := m1); auto.
-          destruct H0. rewrite H0. rewrite Properties.map.putmany_comm.
-          * apply Properties.map.sub_domain_putmany_r. apply Properties.map.sub_domain_refl.
-          * auto.
-      - split; auto. unfold R_putmany. auto.
-Qed.
-
-Local Infix " a +m b" := (Interface.map.putmany a b) (at level 11).
+Definition R_putmany (m1 m2 m : @Interface.map.rep (@word (@semantics Defaults64.default_parameters))
+Init.Byte.byte (@mem (@semantics Defaults64.default_parameters))) := m = Interface.map.putmany m1 m2.
 
 Lemma split_distr (m m1 m2 : @Interface.map.rep (@word (@semantics Defaults64.default_parameters))
 Init.Byte.byte (@mem (@semantics Defaults64.default_parameters))) x x0 x1 x2 : msplit m m1 m2 -> msplit m1 x x0 -> msplit m2 x1 x2
@@ -510,31 +465,6 @@ Proof.
     }
 Qed.
 
-        
-
- Lemma alloc_seps_alt (m m1 m2 : @Interface.map.rep (@word (@semantics Defaults64.default_parameters))
-    Init.Byte.byte (@mem (@semantics Defaults64.default_parameters)))
-    P1 R1 P2 R2 : Interface.map.split m m1 m2 ->
-      (P1 * R1)%sep m1 -> (P2 * R2)%sep m2 ->
-        exists (R' : Interface.map.rep -> Prop), (P1 * P2 * R')%sep m.
-Proof.
-  intros. destruct H0. destruct H0. destruct H0. destruct H2.
-          destruct H1. destruct H1. destruct H1. destruct H4.
-          exists (R_putmany x0 x2). unfold sep. exists (Interface.map.putmany x x1).
-          exists (Interface.map.putmany x0 x2). split.
-            - pose proof (split_distr m m1 m2 x x0 x1 x2). apply H6; auto.
-            - split.
-              + exists x. exists x1. split; auto. destruct H1. unfold msplit. split; auto.
-                destruct H0. apply Properties.map.sub_domain_disjoint with (m1' := m1).
-                * rewrite Properties.map.disjoint_comm. apply Properties.map.sub_domain_disjoint with (m1' := m2).
-                  {
-                    rewrite Properties.map.disjoint_comm; auto. destruct H. auto.
-                  }
-                  rewrite H1. apply Properties.map.sub_domain_putmany_r. apply Properties.map.sub_domain_refl.
-                * rewrite H0. apply Properties.map.sub_domain_putmany_r. apply Properties.map.sub_domain_refl.
-              + unfold R_putmany. auto.
-Qed.
-
 Lemma alloc_seps_alt' (m m1 m2 : @Interface.map.rep (@word (@semantics Defaults64.default_parameters))
 Init.Byte.byte (@mem (@semantics Defaults64.default_parameters)))
 P1 P2 : Interface.map.split m m1 m2 ->
@@ -563,628 +493,185 @@ Qed.
 Require Import WordByWordMontgomery.
 Require Import coqutil.Map.Properties.
 
-Lemma Bignum_anybytes: forall m a wa, Bignum n a wa m -> anybytes a (Z.of_nat n * 8) m.
+Lemma Bignum_anybytes: forall m a wa, Bignum n a wa m -> anybytes a (num_bytes) m.
 Proof.
   intros. pose proof (Bignum_to_bytes n a wa).
   unfold impl1 in H0.
   pose proof (H0 m H). unfold ex1 in H1. destruct H1.
   pose proof (array_1_to_anybytes x m a). sepsimpl_hyps. apply H2 in H3.
-  assert (Z.of_nat n * 8 = Z.of_nat (Datatypes.length x)).
+  assert (num_bytes = Z.of_nat (Datatypes.length x)).
   {
     rewrite H1. simpl. auto.
   }
   rewrite H4. auto.
 Qed.
 
-Lemma anybytes_Bignum: forall m a, anybytes a (Z.of_nat n * 8) m -> exists wa, (Bignum n a wa) m.
+Lemma anybytes_Bignum: forall m a, anybytes a (num_bytes) m -> exists wa, (Bignum n a wa) m.
 Proof.
   intros. About anybytes. destruct H.
-  pose proof (Bignum_of_bytes 6 a x). assert (length x =  (6 * (Z.to_nat word_size_in_bytes))%nat).
+  pose proof (Bignum_of_bytes n a x). assert (length x =  (n * (Z.to_nat word_size_in_bytes))%nat).
     {
-      simpl. simpl in H. Check ftprint. pose proof (map.of_disjoint_list_zip_length (ftprint a 48) x m).
+      simpl. simpl in H. Check ftprint. pose proof (map.of_disjoint_list_zip_length (ftprint a num_bytes) x m).
       simpl in H1. rewrite H1; auto.
     }
   apply H0 in H1. unfold impl1 in H1. unfold ex1 in H1.
-  pose proof (of_disjoint_list_zip_to_array_1 (n * 8) a x m). apply H2 in H.
-  assert (n = 6)%nat by auto. rewrite H3. apply H1. auto.
+  pose proof (of_disjoint_list_zip_to_array_1 (Z.to_nat num_bytes) a x m). apply H2 in H.
+  apply H1. auto.
 Qed.
 
-Lemma anybytes_Bignum_alt: forall m a R, ((anybytes a (Z.of_nat n * 8)) * R)%sep m 
-  -> exists wa, (Bignum n a wa * R)%sep m.
+Lemma empty_frame: forall (P : (@Interface.map.rep (@word (@semantics Defaults64.default_parameters))
+Init.Byte.byte (@mem (@semantics Defaults64.default_parameters))) -> Prop) (m : (@Interface.map.rep (@word (@semantics Defaults64.default_parameters))
+Init.Byte.byte (@mem (@semantics Defaults64.default_parameters)))),
+P m -> exists R, (P * R)%sep m.
+Proof. intros. exists (emp True). ecancel_assumption. Qed.
+
+Lemma sep_assoc_proj1 (m : @Interface.map.rep (@word (@semantics Defaults64.default_parameters))
+Init.Byte.byte (@mem (@semantics Defaults64.default_parameters))) P Q R : ((P * Q) * R)%sep m -> (P * (Q * R))%sep m.
 Proof.
-  intros. do 3 destruct H. destruct H0.
-  pose proof (anybytes_Bignum x a H0). destruct H2.
-  exists x1.
-  exists x. exists x0. split; auto.
+  apply (sep_assoc _ _ _ m).
+Qed. 
+
+Lemma sep_assoc_proj2 (m : @Interface.map.rep (@word (@semantics Defaults64.default_parameters))
+Init.Byte.byte (@mem (@semantics Defaults64.default_parameters))) P Q R : (P * (Q * R))%sep m -> (P * Q * R)%sep m.
+Proof.
+  apply (sep_assoc _ _ _ m).
+Qed. 
+
+Notation montsub a b c :=
+  ((eval (from_mont (a))) mod m =
+      (eval (from_mont (b)) -
+       eval (from_mont (c))) mod m).
+
+Notation montadd a b c :=
+  ((eval (from_mont (a))) mod m =
+      (eval (from_mont (b)) +
+       eval (from_mont (c))) mod m).
+
+Notation montmul a b c :=
+  ((eval (from_mont (a))) mod m =
+      (eval (from_mont (b)) *
+       eval (from_mont (c))) mod m).
+
+Lemma postcond_from_precond xr xi yr yi resr resi x1 x2 x3 x4 x5 x6:
+  montsub resi x1 x2 -> valid resi -> valid x1 -> valid x2
+  -> montsub x1 x3 x4 -> montmul x3 x5 x6 -> valid x3 -> valid x6
+  -> montadd x6 yr yi -> valid x5 -> montadd x5 xr xi -> valid resr
+  -> montsub resr x4 x2 -> montmul x2 xi yi -> valid x4 -> montmul x4 xr yr
+  -> valid xr -> valid xi -> valid yr -> valid yi
+-> Fp2_mul_Gallina_spec (xr, xi) (yr, yi) (resr, resi).
+Proof.
+  intros. unfold Fp2_mul_Gallina_spec.
+  split; [auto|].
+  split; [auto|]. split.
+                    - repeat rewrite Prod.fst_pair; repeat rewrite Prod.snd_pair.
+                      rewrite (valid_mod H10) in H11; rewrite H11.
+                      rewrite (valid_mod H13) in H14; rewrite H14.
+                      rewrite (valid_mod H2) in H12; rewrite H12.
+                        rewrite <- Zminus_mod. apply (f_equal (fun y => y mod m)). ring.
+                    - repeat rewrite Prod.fst_pair; repeat rewrite Prod.snd_pair.
+                      rewrite (valid_mod H0) in H; rewrite H.
+                      rewrite (valid_mod H1) in H3; rewrite H3.
+                      rewrite (valid_mod H5) in H4; rewrite H4.
+                      rewrite (valid_mod H8) in H9; rewrite H9.
+                      rewrite (valid_mod H6) in H7; rewrite H7.
+                      rewrite (valid_mod H13) in H14; rewrite H14.
+                      rewrite (valid_mod H2) in H12; rewrite H12.
+                      rewrite <- Z.mul_mod.
+                        2: { unfold m. simpl. auto with zarith. }
+                        remember (eval (from_mont xr)) as xr'.
+                        remember (eval (from_mont yr)) as yr'.
+                        rewrite <- (Zminus_mod ( _ * _)).
+                      rewrite <- Zminus_mod. apply (f_equal (fun y => (y mod m))). ring.
 Qed.
 
+(*We can now write the tactics needed to automate proofs.*)
+
+Ltac mytac := lazymatch goal with
+| [
+    |- exists (_ _ : @Interface.map.rep _ _ _),
+      (anybytes ?addr _ _) /\ (msplit ?mem _ _) /\ _ ] =>
+      repeat match goal with 
+      | [ H : (?Rl * ((Bignum _ addr ?aval) * ?Rr))%sep mem |- _ ] => 
+        let Ha := (fresh "Ha") in
+        let m := fresh "m" in
+        let mStack := fresh "mStack" in
+        assert (Ha : ((Bignum n addr aval) * (Rl * Rr))%sep mem) by ecancel_assumption;
+        destruct Ha as [mStack [m [? []]]];
+        exists m; exists mStack; split; [ eapply Bignum_anybytes; eassumption | split; [apply Properties.map.split_comm; auto|]]
+        
+      | [ H : _ mem |- _ ] => apply (sep_assoc_proj2 mem) in H
+      end
+end.
+
+Ltac straightline' :=
+  match goal with
+  | [Hminit : ?mcond (?minit : @Interface.map.rep _ _ _)
+      |- forall (_ : @word.rep _ _)
+                (_ _ : @Interface.map.rep _ _ _),
+          anybytes _ ?numbytes _ -> msplit _ ?minit _ -> _ ] =>
+      let a := (fresh "a") in
+      let mStack := (fresh "mStack") in
+      let mnew := (fresh "mnew") in
+      let Hany := (fresh "Hany") in
+      let HanyBignum := (fresh "HanyBignum") in
+      let anyval := (fresh "anyval") in
+      let Hsplit := (fresh "Hsplit") in
+      let Hmnew := (fresh "Hmnew") in
+      let R := (fresh "R") in
+      intros a mStack mnew Hany Hsplit; destruct (anybytes_Bignum mStack a Hany) as [anyval HanyBignum];
+      destruct (alloc_seps_alt' mnew minit mStack mcond (Bignum _ _ _) Hsplit (empty_frame mcond minit Hminit) (empty_frame (Bignum _ _ _) mStack HanyBignum)) as [R Hmnew];
+      clear Hany Hsplit HanyBignum
+  | _ => straightline
+  end.
 
 Require Import coqutil.Tactics.letexists.
 Theorem Fp2_mul_ok: program_logic_goal_for_function! Fp2_mul.
 Proof.
-  straightline. straightline. straightline.
-  straightline. straightline. straightline. straightline. straightline. straightline.
-  straightline. straightline. straightline. straightline. straightline. straightline. straightline.
-  straightline. straightline.
-  straightline. straightline. straightline. straightline. straightline.
-  About handle_call.
-          remember ((Bignum n pxr wxr * Bignum n pxi wxi * Bignum n pyr wyr *
-          Bignum n pyi wyi * Bignum n poutr wold_outr * 
-          Bignum n pouti wold_outi)%sep) as Hm0.
+  (*Handle parts of function up until function calls.
+    We use a modified version of Bedrock2's straightline tactic.
+    This version  undoes the fragmentation of memory in the context
+    done by stack allocation.*)
+  repeat straightline'.
 
-          (*Bring into context array pointed to by pxi*)
-          pose proof (alloc_seps mCombined1 mCombined0 mStack1 Hm0 H17).
-          assert (exists R : Interface.map.rep -> Prop, (Hm0 * R)%sep mCombined0).
-            {
-              pose proof (alloc_seps mCombined0 mCombined mStack0 Hm0 H15).
-              assert (exists R : Interface.map.rep -> Prop, (Hm0 * R)%sep mCombined).
-                {
-                  pose proof (alloc_seps mCombined m0 mStack Hm0 H13).
-                  assert (exists R : Interface.map.rep -> Prop, (Hm0 * R)%sep m0).
-                    {
-                      exists (emp True). sepsimpl; auto.
-                    }
-                  apply H20 in H21. auto.
-                }
-              apply H19 in H20. auto.
-            } apply H18 in H19. destruct H19.
-            
-            (*Bring into context array pointed to by a*)
-            Check anybytes.
-            (* apply anybytes_Bignum in H12. destruct H12.
-            apply anybytes_Bignum in H14. destruct H14.
-            apply anybytes_Bignum in H16. destruct H16. *)
-            pose proof (alloc_seps_alt' mCombined1 mCombined0 mStack1 ((anybytes a0 48) * (anybytes a 48) * Hm0)%sep (anybytes a1 48) H17).
-            assert (exists R : Interface.map.rep -> Prop, ( (anybytes a0 48) * (anybytes a 48 * Hm0) * R)%sep mCombined0).
-              { pose proof (alloc_seps_alt' mCombined0 mCombined mStack0 ((anybytes a 48) * Hm0)%sep (anybytes a0 48) H15).
-                assert (exists R : Interface.map.rep -> Prop, (anybytes a 48 * Hm0 * R)%sep mCombined).
-                  {
-                    apply map.split_comm in H13.
-                    pose proof (alloc_seps_alt' mCombined mStack m0 (anybytes a 48) Hm0 H13).
-                    assert (exists R : Interface.map.rep -> Prop, (anybytes a 48 * R)%sep mStack).
-                      {
-                         exists (emp True). sepsimpl; auto.
-                      }
-                    assert (exists R : Interface.map.rep -> Prop, (Hm0 * R)%sep m0).
-                      {
-                        exists (emp True). sepsimpl; auto.
-                      }
-                    apply H22 in H23.
-                     2: {auto. }
-                    
-                    
-                    auto.
-                  }
-                assert (exists R : Interface.map.rep -> Prop, ((anybytes a0 48) * R)%sep mStack0).
-                {
-                  exists (emp True). sepsimpl; auto.
-                }
-                apply H21 in H22; auto. destruct H22. eexists. ecancel_assumption.
-              }
-            assert (exists R : Interface.map.rep -> Prop, ((anybytes a1 48) * R)%sep mStack1).
-              {
-                exists (emp True). sepsimpl; auto.
-              }
-            
-            assert (exists R' : Interface.map.rep -> Prop,
-              (anybytes a0 48 * anybytes a 48 * Hm0 * anybytes a1 48 * R')%sep mCombined1).
-                {
-                  apply H20.
-                  - destruct H21. eexists. ecancel_assumption.
-                  - destruct H22; eexists; ecancel_assumption.
-                }
-              destruct H23.
-            (*Bring into context array pointed to by pyi*)
-            (* pose proof (alloc_seps mCombined1 mCombined0 mStack1 Hm0 H17).
-          assert (exists R : Interface.map.rep -> Prop, (Hm0 * R)%sep mCombined0).
-            {
-              pose proof (alloc_seps mCombined0 mCombined mStack0 Hm0 H15).
-              assert (exists R : Interface.map.rep -> Prop, (Hm0 * R)%sep mCombined).
-                {
-                  pose proof (alloc_seps mCombined m0 mStack Hm0 H13).
-                  assert (exists R : Interface.map.rep -> Prop, (Hm0 * R)%sep m0).
-                    {
-                      exists (emp True ). sepsimpl; auto.
-                    }
-                  apply H24 in H25. auto.
-                }
-              apply H23 in H24. auto.
-            } apply H22 in H23. destruct H23. *)
-            rewrite HeqHm0 in H23.
+  (*Handle function calls.
+    Note that the use of the "auto" tactic here is to handle preconditions af callees.
+    In this case auto is sufficient, but for more complicated function calls
+    this should be done manually.*)
+  repeat (handle_call; [auto| auto| ]).
 
-            (*Rephrasing seperation hypothesis to Bignum instead of anybytes.*)
-            remember ((anybytes a 48 *
-            (Bignum n pxr wxr * Bignum n pxi wxi * Bignum n pyr wyr *
-             Bignum n pyi wyi * Bignum n poutr wold_outr *
-             Bignum n pouti wold_outi) * anybytes a1 48 * x0)%sep) as Ra0.
-            assert ( (anybytes a0 48 * Ra0)%sep mCombined1).
-              {
-                 subst Ra0; ecancel_assumption.
-              }
-              pose proof (anybytes_Bignum_alt mCombined1 a0 Ra0). assert (Z.of_nat n * 8 = 48) by auto. rewrite H26 in H25.
-               apply H25 in H24. destruct H24.
-               
-                subst Ra0.
+  (*Fragmentation of the memorr after function body is necessary for stack allocation
+    to ensure that output and intermediate variables are stored correctly in memory
+    TODO: find a better name for this tactic.*)
+  repeat mytac.
+  
+  (* Handle parts of function up until proving the postcondition*)
+  repeat straightline'.
 
-               remember ((Bignum n a0 x1 *
-               (Bignum n pxr wxr * Bignum n pxi wxi * Bignum n pyr wyr *
-                Bignum n pyi wyi * Bignum n poutr wold_outr *
-                Bignum n pouti wold_outi) * anybytes a1 48 * x0)%sep) as Ra.
-               assert ((anybytes a 48 * Ra)%sep mCombined1).
-               {
-                 subst Ra; ecancel_assumption.
-               }
-               pose proof (anybytes_Bignum_alt mCombined1 a Ra). assert (Z.of_nat n * 8 = 48) by auto. rewrite H29 in H28.
-                apply H28 in H27. destruct H27.
+  (*Postcondition is proved
+    reflexivity solves first part; which will always be the case when no complicated
+    reasoning about separation logic is needed, i.e. when the seperating conjuction is
+    used only as a means of referencing memory. *)
+  split; [reflexivity| split; [reflexivity |]].
+  
+  (*evars introduced and instantiated.
+    The instantiation is done by Bedrock2's ecancel_assumption tactic.*)
+  do 3 eexists; split; [|ecancel_assumption].
 
-                subst Ra.
+  (*It remains only to show the non-Bedrock2 specific parts of the postcondition.
+    some is done by auto.*)
+  split; [| auto].
 
-                 remember ((Bignum n a0 x1 * Bignum n a x2 *
-                (Bignum n pxr wxr * Bignum n pxi wxi * Bignum n pyr wyr *
-                 Bignum n pyi wyi * Bignum n poutr wold_outr *
-                 Bignum n pouti wold_outi) * x0)%sep) as Ra1.
-                assert ( (anybytes a1 48 * Ra1)%sep mCombined1).
-                {
-                  subst Ra1; ecancel_assumption.
-                }
-                pose proof (anybytes_Bignum_alt mCombined1 a1 Ra1). assert (Z.of_nat n * 8 = 48) by auto. rewrite H32 in H31.
-                 apply H31 in H30. destruct H30.
-                subst Ra1. clear H27. clear H24.          
+  (*We have proved that the Gallina specification is met in a separate lemma: postcond_from_precond.
+    A more natural approach would be to prove the precondition directly here.
+    We use a lemma to illustrate the fact that proving the non-Bedrock2 specific parts of
+    the postcondition is separated from the Bedrock2 specific parts, which are mostly automated.*)
+  apply (postcond_from_precond (map word.unsigned wxr) (map word.unsigned wxi) (map word.unsigned wyr) (map word.unsigned wyi) (map word.unsigned x1) (map word.unsigned x6)
+  (map word.unsigned x5) (map word.unsigned x0) (map word.unsigned x4) (map word.unsigned x) 
+  (map word.unsigned x2) (map word.unsigned x3) 
+  ); auto.
+  Qed.
 
-
-            straightline_call.
-            2: { ecancel_assumption. }
-            3: { ecancel_assumption. }
-            2: { ecancel_assumption. }
-            1: { auto. }
-            repeat straightline.
-
-(* 
-            remember ((emp
-            (eval (from_mont (map word.unsigned x5)) mod m =
-             (eval (from_mont (map word.unsigned wxi)) *
-              eval (from_mont (map word.unsigned wyi))) mod m /\
-             valid (map word.unsigned x5)) * Ra)%sep) as Ra'.
-            assert ((anybytes a 48 * Ra')%sep mCombined1).
-            {
-              subst Ra; ecancel_assumption.
-            }
-            pose proof (anybytes_Bignum_alt mCombined1 a Ra). assert (Z.of_nat n * 8 = 48) by auto. rewrite H29 in H28.
-             apply H28 in H27. destruct H27. *)
-
-
-            straightline_call.
-            2: {
-              sepsimpl_hyps. subst Hm0. ecancel_assumption. 
-            }
-            2: { sepsimpl_hyps. subst Hm0. ecancel_assumption. }
-            2: { sepsimpl_hyps. subst Hm0. sepsimpl_hyps. ecancel_assumption. }
-            1: { auto. }
-            repeat straightline.
-            straightline_call.
-            2: {ecancel_assumption. }
-            2: { ecancel_assumption. }
-            2: { ecancel_assumption. }
-            1: { sepsimpl_hyps. auto. }
-            repeat straightline.
-            straightline_call.
-            2, 3:  ecancel_assumption.
-            2: { ecancel_assumption. }
-            1: auto.
-            repeat straightline. straightline_call.
-            2, 3, 4: ecancel_assumption.
-            1: auto.
-            repeat straightline; straightline_call.
-            2, 3, 4: ecancel_assumption.
-            1: sepsimpl_hyps; auto.
-            repeat straightline; straightline_call.
-            2, 3, 4: ecancel_assumption.
-            1: sepsimpl_hyps; auto.
-            repeat straightline. straightline_call.
-            2, 3, 4: ecancel_assumption.
-            1: sepsimpl_hyps; auto.
-            repeat straightline.
-            sepsimpl_hyps.
-            remember ((@emp
-            (@word.rep
-               (@width (@semantics Defaults64.default_parameters))
-               (@word (@semantics Defaults64.default_parameters)))
-            Init.Byte.byte
-            (@mem (@semantics Defaults64.default_parameters))
-            (and
-               (@eq Z
-                  (Z.modulo
-                     (@WordByWordMontgomery.eval
-                        (@width
-                           (@semantics Defaults64.default_parameters))
-                        (WordByWordMontgomery.n bls12prime.m
-                           (@width
-                              (@semantics Defaults64.default_parameters)))
-                        (WordByWordMontgomery.from_montgomerymod
-                           (@width
-                              (@semantics Defaults64.default_parameters))
-                           (WordByWordMontgomery.n bls12prime.m
-                              (@width
-                                 (@semantics
-                                    Defaults64.default_parameters)))
-                           bls12prime.m
-                           (WordByWordMontgomery.m' bls12prime.m
-                              (@width
-                                 (@semantics
-                                    Defaults64.default_parameters)))
-                           (@map
-                              (@word.rep
-                                 (@width
-                                    (@semantics
-                                       Defaults64.default_parameters))
-                                 (@word
-                                    (@semantics
-                                       Defaults64.default_parameters)))
-                              Z
-                              (@word.unsigned
-                                 (@width
-                                    (@semantics
-                                       Defaults64.default_parameters))
-                                 (@word
-                                    (@semantics
-                                       Defaults64.default_parameters)))
-                              x8))) bls12prime.m)
-                  (Z.modulo
-                     (Z.sub
-                        (@WordByWordMontgomery.eval
-                           (@width
-                              (@semantics Defaults64.default_parameters))
-                           (WordByWordMontgomery.n bls12prime.m
-                              (@width
-                                 (@semantics
-                                    Defaults64.default_parameters)))
-                           (WordByWordMontgomery.from_montgomerymod
-                              (@width
-                                 (@semantics
-                                    Defaults64.default_parameters))
-                              (WordByWordMontgomery.n bls12prime.m
-                                 (@width
-                                    (@semantics
-                                       Defaults64.default_parameters)))
-                              bls12prime.m
-                              (WordByWordMontgomery.m' bls12prime.m
-                                 (@width
-                                    (@semantics
-                                       Defaults64.default_parameters)))
-                              (@map
-                                 (@word.rep
-                                    (@width
-                                       (@semantics
-                                          Defaults64.default_parameters))
-                                    (@word
-                                       (@semantics
-                                          Defaults64.default_parameters)))
-                                 Z
-                                 (@word.unsigned
-                                    (@width
-                                       (@semantics
-                                          Defaults64.default_parameters))
-                                    (@word
-                                       (@semantics
-                                          Defaults64.default_parameters)))
-                                 x6)))
-                        (@WordByWordMontgomery.eval
-                           (@width
-                              (@semantics Defaults64.default_parameters))
-                           (WordByWordMontgomery.n bls12prime.m
-                              (@width
-                                 (@semantics
-                                    Defaults64.default_parameters)))
-                           (WordByWordMontgomery.from_montgomerymod
-                              (@width
-                                 (@semantics
-                                    Defaults64.default_parameters))
-                              (WordByWordMontgomery.n bls12prime.m
-                                 (@width
-                                    (@semantics
-                                       Defaults64.default_parameters)))
-                              bls12prime.m
-                              (WordByWordMontgomery.m' bls12prime.m
-                                 (@width
-                                    (@semantics
-                                       Defaults64.default_parameters)))
-                              (@map
-                                 (@word.rep
-                                    (@width
-                                       (@semantics
-                                          Defaults64.default_parameters))
-                                    (@word
-                                       (@semantics
-                                          Defaults64.default_parameters)))
-                                 Z
-                                 (@word.unsigned
-                                    (@width
-                                       (@semantics
-                                          Defaults64.default_parameters))
-                                    (@word
-                                       (@semantics
-                                          Defaults64.default_parameters)))
-                                 x7)))) bls12prime.m))
-               (WordByWordMontgomery.valid
-                  (@width (@semantics Defaults64.default_parameters))
-                  (WordByWordMontgomery.n bls12prime.m
-                     (@width (@semantics Defaults64.default_parameters)))
-                  bls12prime.m
-                  (@map
-                     (@word.rep
-                        (@width
-                           (@semantics Defaults64.default_parameters))
-                        (@word
-                           (@semantics Defaults64.default_parameters)))
-                     Z
-                     (@word.unsigned
-                        (@width
-                           (@semantics Defaults64.default_parameters))
-                        (@word
-                           (@semantics Defaults64.default_parameters)))
-                     x8))))) as emp1.
-                     remember ((@emp
-                     (@word.rep
-                        (@width (@semantics Defaults64.default_parameters))
-                        (@word (@semantics Defaults64.default_parameters)))
-                     Init.Byte.byte
-                     (@mem (@semantics Defaults64.default_parameters))
-                     (and
-                        (@eq Z
-                           (Z.modulo
-                              (@WordByWordMontgomery.eval
-                                 (@width
-                                    (@semantics
-                                       Defaults64.default_parameters))
-                                 (WordByWordMontgomery.n bls12prime.m
-                                    (@width
-                                       (@semantics
-                                          Defaults64.default_parameters)))
-                                 (WordByWordMontgomery.from_montgomerymod
-                                    (@width
-                                       (@semantics
-                                          Defaults64.default_parameters))
-                                    (WordByWordMontgomery.n bls12prime.m
-                                       (@width
-                                          (@semantics
-                                             Defaults64.default_parameters)))
-                                    bls12prime.m
-                                    (WordByWordMontgomery.m' bls12prime.m
-                                       (@width
-                                          (@semantics
-                                             Defaults64.default_parameters)))
-                                    (@map
-                                       (@word.rep
-                                          (@width
-                                             (@semantics
-                                               Defaults64.default_parameters))
-                                          (@word
-                                             (@semantics
-                                               Defaults64.default_parameters)))
-                                       Z
-                                       (@word.unsigned
-                                          (@width
-                                             (@semantics
-                                               Defaults64.default_parameters))
-                                          (@word
-                                             (@semantics
-                                               Defaults64.default_parameters)))
-                                       x7))) bls12prime.m)
-                           (Z.modulo
-                              (Z.mul
-                                 (@WordByWordMontgomery.eval
-                                    (@width
-                                       (@semantics
-                                          Defaults64.default_parameters))
-                                    (WordByWordMontgomery.n bls12prime.m
-                                       (@width
-                                          (@semantics
-                                             Defaults64.default_parameters)))
-                                    (WordByWordMontgomery.from_montgomerymod
-                                       (@width
-                                          (@semantics
-                                             Defaults64.default_parameters))
-                                       (WordByWordMontgomery.n bls12prime.m
-                                          (@width
-                                             (@semantics
-                                               Defaults64.default_parameters)))
-                                       bls12prime.m
-                                       (WordByWordMontgomery.m'
-                                          bls12prime.m
-                                          (@width
-                                             (@semantics
-                                               Defaults64.default_parameters)))
-                                       (@map
-                                          (@word.rep
-                                             (@width
-                                               (@semantics
-                                               Defaults64.default_parameters))
-                                             (@word
-                                               (@semantics
-                                               Defaults64.default_parameters)))
-                                          Z
-                                          (@word.unsigned
-                                             (@width
-                                               (@semantics
-                                               Defaults64.default_parameters))
-                                             (@word
-                                               (@semantics
-                                               Defaults64.default_parameters)))
-                                          wxi)))
-                                 (@WordByWordMontgomery.eval
-                                    (@width
-                                       (@semantics
-                                          Defaults64.default_parameters))
-                                    (WordByWordMontgomery.n bls12prime.m
-                                       (@width
-                                          (@semantics
-                                             Defaults64.default_parameters)))
-                                    (WordByWordMontgomery.from_montgomerymod
-                                       (@width
-                                          (@semantics
-                                             Defaults64.default_parameters))
-                                       (WordByWordMontgomery.n bls12prime.m
-                                          (@width
-                                             (@semantics
-                                               Defaults64.default_parameters)))
-                                       bls12prime.m
-                                       (WordByWordMontgomery.m'
-                                          bls12prime.m
-                                          (@width
-                                             (@semantics
-                                               Defaults64.default_parameters)))
-                                       (@map
-                                          (@word.rep
-                                             (@width
-                                               (@semantics
-                                               Defaults64.default_parameters))
-                                             (@word
-                                               (@semantics
-                                               Defaults64.default_parameters)))
-                                          Z
-                                          (@word.unsigned
-                                             (@width
-                                               (@semantics
-                                               Defaults64.default_parameters))
-                                             (@word
-                                               (@semantics
-                                               Defaults64.default_parameters)))
-                                          wyi)))) bls12prime.m))
-                        (WordByWordMontgomery.valid
-                           (@width
-                              (@semantics Defaults64.default_parameters))
-                           (WordByWordMontgomery.n bls12prime.m
-                              (@width
-                                 (@semantics Defaults64.default_parameters)))
-                           bls12prime.m
-                           (@map
-                              (@word.rep
-                                 (@width
-                                    (@semantics
-                                       Defaults64.default_parameters))
-                                 (@word
-                                    (@semantics
-                                       Defaults64.default_parameters))) Z
-                              (@word.unsigned
-                                 (@width
-                                    (@semantics
-                                       Defaults64.default_parameters))
-                                 (@word
-                                    (@semantics
-                                       Defaults64.default_parameters))) x7))))) as emp2.
-
-            remember (emp1 *
-            (Bignum n poutr x8 *
-             (emp2 *
-              (Bignum n a0 x7 *
-               (Bignum n a x6 *
-                (Bignum n pxr wxr *
-                 (Bignum n pxi wxi * (Bignum n pyr wyr * (Bignum n pyi wyi * x0)))))))) *
-           Bignum n pouti x13)%sep as Ra11.
-
-            assert ((Bignum n a1 x9 * Ra11)%sep a11 ).
-              {
-                subst Ra11. ecancel_assumption.
-              }
-              destruct H79. destruct H79. exists x15. exists x14. split.
-              1: {
-                apply Bignum_anybytes with (wa := x9). destruct H79. destruct H80.
-                auto.
-              }
-              split.
-              1: {
-                apply Properties.map.split_comm. destruct H79. auto.
-              }
-              destruct H79. destruct H80.
-              subst Ra11.
-              remember ((emp1 *
-              (Bignum n poutr x8 *
-               (emp2 *
-                 (Bignum n a x6 *
-                  (Bignum n pxr wxr *
-                   (Bignum n pxi wxi * (Bignum n pyr wyr * (Bignum n pyi wyi * x0))))))) *
-              Bignum n pouti x13)%sep) as Rx15.
-              assert ((Bignum n a0 x7 * Rx15)%sep x15).
-              {
-                subst Rx15. ecancel_assumption.
-              }
-              destruct H82. destruct H82. destruct H82. destruct H83.
-              exists x17. exists x16. split.
-              1: {
-                apply Bignum_anybytes with (wa := x7). auto.
-              }
-              split.
-              1: {
-                apply Properties.map.split_comm. auto.
-              }
-              subst Rx15.
-              remember ((emp1 *
-              (Bignum n poutr x8 *
-               (emp2 *
-                  (Bignum n pxr wxr *
-                   (Bignum n pxi wxi * (Bignum n pyr wyr * (Bignum n pyi wyi * x0)))))) *
-              Bignum n pouti x13)%sep) as Rx17.
-              assert ((Bignum n a x6 * Rx17)%sep x17).
-              {
-                subst Rx17. ecancel_assumption.
-              }
-              destruct H85. destruct H85. destruct H85. destruct H86.
-              exists x19. exists x18. split.
-              1: {
-                apply Bignum_anybytes with (wa := x6). auto.
-              }
-              split.
-              1: {
-                apply Properties.map.split_comm. auto.
-              }
-              subst Rx17.
-              repeat straightline. split.
-               1: { reflexivity. }
-               split.
-               1: {reflexivity. }
-               eexists. eexists. eexists. split.
-               2: { ecancel_assumption. }
-               unfold Fp2_mul_Gallina_spec.
-               split; split.
-               all: sepsimpl_hyps.
-                - subst emp1. sepsimpl_hyps. auto.
-                - split.
-                  + subst emp2. subst emp1. sepsimpl_hyps. auto.
-                  + split.
-                    * subst emp1. subst emp2.
-                      sepsimpl_hyps.
-                      remember (eval (from_mont (map word.unsigned wxi))) as xi.
-                      remember (eval (from_mont (map word.unsigned wxr))) as xr.
-                      remember (eval (from_mont (map word.unsigned wyi))) as yi.
-                      remember (eval (from_mont (map word.unsigned wyr))) as yr.
-                      rewrite (valid_mod H89) in H84. rewrite H84.
-                  
-                        rewrite (valid_mod H78) in H49. rewrite H49.
-                        rewrite (valid_mod H54) in H33. rewrite H33.
-                        rewrite <- Zminus_mod. apply (f_equal (fun y => y mod m)). ring.
-                    * subst emp1. subst emp2. sepsimpl_hyps.
-                      remember (eval (from_mont (map word.unsigned wxi))) as xi.
-                      remember (eval (from_mont (map word.unsigned wxr))) as xr.
-                      remember (eval (from_mont (map word.unsigned wyi))) as yi.
-                      remember (eval (from_mont (map word.unsigned wyr))) as yr.
-                      rewrite (valid_mod H40) in H24. rewrite H24.
-                      rewrite (valid_mod H56) in H27. rewrite H27.
-                      rewrite (valid_mod H58) in H55. rewrite H55.
-                      rewrite (valid_mod H62) in H59. rewrite H59.
-                      rewrite (valid_mod H60) in H57. rewrite H57.
-                      rewrite (valid_mod H54) in H33. rewrite H33.
-                      rewrite (valid_mod H78) in H49. rewrite H49.
-                      rewrite <- Z.mul_mod; [| unfold m; lia].
-                      rewrite <- (Zminus_mod _ (xr * yr)).
-                      rewrite <- Zminus_mod. apply (f_equal (fun y => (y mod m))). ring.
-                      
-                      
-                      
-                - subst emp1; subst emp2; sepsimpl_hyps; auto.
-                - subst emp1; subst emp2. sepsimpl_hyps. auto.
-Qed.
-
-(*Printing to C*)
+(*Printing to C
 From bedrock2 Require Import ToCString Bytedump.
 Definition bls12_c_add :=
   c_module (add :: nil).
@@ -1195,6 +682,5 @@ Definition bls12_c_add :=
   Definition bls12_c_Fp2_add :=
   c_module (Fp2_add :: nil).
   Definition bls12_c_Fp2_mul :=
-  c_module (Fp2_mul :: nil).
-Eval compute in bls12_c_Fp2_mul.
+  c_module (Fp2_mul :: nil). *)
 
